\section{Incremental PID controller}
The discrete PID controller is defined as follows:
\begin{equation}
    u(n)=k_p e(n)+k_i\sum_{k=0}^{n}e(k)+k_d[e(n)-e(n-1)]
\end{equation}
In order to switch to the incremental PID controller expression,
\begin{equation}
    \Delta u(n)=u(n)-u(n-1)
\end{equation}
is defined. Plugging in the controller results in,
\begin{equation}
\begin{split}
    \Delta u(n)&=u(n)-u(n-1)\\
    &=k_p e(n)+k_i\sum_{k=0}^{n}e(k)+k_d[e(n)-e(n-1)]-k_p e(n-1)\\
     &-k_i\sum_{k=0}^{n-1}e(k)-k_d[e(n-1)-e(n-2)]\\
    &=k_p e(n)+k_i\sum_{k=0}^{n-1}e(k)+k_ie(n)+k_de(n)-k_de(n-1)\\
    &-k_p e(n-1)-k_i\sum_{k=0}^{n-1}e(k-1)-k_de(n-1)+k_de(n-2)\\
    &=k_p e(n)-k_p e(n-1)+k_ie(n)+k_de(n)-2k_de(n-1)+k_de(n-2)\\
    &=k_p [e(n)-e(n-1)]+k_ie(n)+k_d[e(n)-2e(n-1)+e(n-2)]
\end{split}
\end{equation}

\section{Fuzzy PI controller}
Let the inputs be $e(n)$ and $\Delta e(n)$ and the output be $\Delta u(n)$ defined as error, change in error and change in control signal, respectively. 
\input{fig1}
The membership functions Positive(P) and Negative(N) are defined as 
\begin{equation}
    \mu_P(e)\begin{cases}
        0,& e<-L\\
        \frac{e+L}{2L},& -L\leq e\leq L\\
        1,& e>L\\
    \end{cases}\quad
    \mu_N(e)\begin{cases}
        1,& e<-L\\
        \frac{-e+L}{2L},& -L\leq e\leq L\\
        0,& e>L\\
    \end{cases}
\end{equation}
and 
\begin{equation}
    \mu_P(\Delta e)\begin{cases}
        0,& \Delta e<-L\\
        \frac{\Delta e+L}{2L},& -L\leq \Delta e\leq L\\
        1,& \Delta e>L\\
    \end{cases}\quad
    \mu_N(\Delta e)\begin{cases}
        1,& \Delta e<-L\\
        \frac{-\Delta e+L}{2L},& -L\leq \Delta e\leq L\\
        0,& \Delta e>L\\
    \end{cases}
\end{equation}
and depicted in Figure~\ref{fig:fig1}. The membership functions are chosen such that, 
\begin{equation}
    \mu_N(e)+\mu_P(e)=1\quad \mu_N(\Delta e)+\mu_P(\Delta e)=1
\end{equation}

For the output variable the membership function is chosen as
\begin{equation}
    \mu_N(\Delta u)\begin{cases}
        1,& \Delta u=-H\\
        0,& \Delta u\neq-H\\
    \end{cases}\quad
    \mu_P(\Delta u)\begin{cases}
        1,& \Delta u=H\\
        0,& \Delta u\neq H\\
    \end{cases}\quad
    \mu_Z(\Delta u)\begin{cases}
        1,& \Delta u=0\\
        0,& \Delta u\neq 0\\
    \end{cases}
\end{equation}
and is depicted in Figure~\ref{fig:fig2}.
\input{fig2}

\clearpage
\renewcommand{\arraystretch}{1.5} % Vertical padding
The following rule set is constructed.
\begin{table}[h!]
\centering
\caption{Fuzzy Rule Table: Control Output $\Delta u(n)$ based on Error $e(n)$ and Change of Error $\Delta e(n)$}
\begin{tabular}{c@{\hspace{1em}}|@{\hspace{1em}}c@{\hspace{1em}}c@{\hspace{1em}}c}
\toprule
\textbf{$e(n)$ $\backslash$ $\Delta e(n)$} & \textbf{N} & \textbf{Z} & \textbf{P} \\
\midrule
\textbf{N} & N & N & Z \\
\textbf{Z} & N & Z & P \\
\textbf{P} & Z & P & P \\
\bottomrule
\end{tabular}
\end{table}

The rule set is defined as follows:
\begin{quote}
IF $e(n)$ is N AND $\Delta e(n)$ is N THEN output is Negative\\
IF $e(n)$ is N AND $\Delta e(n)$ is P THEN output is Zero\\
IF $e(n)$ is P AND $\Delta e(n)$ is N THEN output is Zero\\
IF $e(n)$ is P AND $\Delta e(n)$ is P THEN output is Positive
\end{quote}

The inference step results in:
\begin{quote}
$\mu_N(e) \mu_N (\Delta e)$ for output $-H$\\
$\mu_N(e) \mu_P (\Delta e)$ for output 0\\
$\mu_P(e) \mu_N (\Delta e)$ for output 0\\
$\mu_P(e) \mu_P (\Delta e)$ for output $H$
\end{quote}
and hence in,
\begin{quote}
$\mu_N(e) \mu_N (\Delta e)$ for output $-H$\\
$\mu_P(e) \mu_P (\Delta e)$ for output $H$
\end{quote}
The defuzzification step gives,
\begin{equation}
    \Delta u(n)=\frac{\mu_P(e) \mu_P (\Delta e)H-\mu_N(e) \mu_N (\Delta e)H}{\mu_N(e) \mu_N (\Delta e)+\mu_N(e) \mu_P (\Delta e)+\mu_P(e) \mu_N (\Delta e)+\mu_P(e) \mu_P (\Delta e)}
\end{equation}
The denominator is simplified as follows:
\begin{equation}
\begin{split}
    \mu_N(e) \mu_N (\Delta e)+\mu_N(e) \mu_P (\Delta e)+\mu_P(e) \mu_N (\Delta e)+\mu_P(e) \mu_P (\Delta e)\\
    =(1-\mu_P(e)) \mu_N (\Delta e)+(1-\mu_P(e)) \mu_P (\Delta e)+\mu_P(e) \mu_N (\Delta e)+\mu_P(e) \mu_P (\Delta e)\\
    =\mu_N (\Delta e)-\mu_P(e)\mu_N (\Delta e)+\mu_P (\Delta e)-\mu_P(e) \mu_P (\Delta e)+\mu_P(e) \mu_N (\Delta e)+\mu_P(e) \mu_P (\Delta e)\\
    =\mu_N (\Delta e)+\mu_P (\Delta e)\\
    =1
\end{split}
\end{equation}
therefore,
\begin{equation}
\begin{split}
    \Delta u(n)&=\mu_P(e) \mu_P (\Delta e)H-\mu_N(e) \mu_N (\Delta e)H\\
    &=H\begin{cases}
    -1,& e<-L\\
    \frac{\Delta e+L}{2L}\frac{e+L}{2L}-\frac{-e+L}{2L}\frac{-\Delta e+L}{2L},& -L\leq e\leq L\\
    1,& e>L\\
    \end{cases}\\
    &=\frac{\Delta e+L}{2L}\frac{e+L}{2L}-\frac{-e+L}{2L}\frac{-\Delta e+L}{2L}\\
    &=\frac{(\Delta e+L)(e+L)-(-e+L)(-\Delta e+L)}{4L^2}\\
    &=\frac{\Delta e(e+L)+L(e+L)-(-e)(-\Delta e+L)-L(-\Delta e+L)}{4L^2}\\
    &=\frac{e\Delta e+L\Delta e+Le+L^2-e\Delta e+Le+L\Delta e-L^2}{4L^2}\\
    &=\frac{L\Delta e+Le+Le+L\Delta e}{4L^2}\\
    &=\frac{2L\Delta e+2Le}{4L^2}\\
    &=\frac{\Delta e+e}{2L}\\
    &=\frac{1}{2L}\Delta e+\frac{1}{2L}e\\
    \Delta u(n)&=\begin{cases}
    -H,& e<-L\\
    \frac{H}{2L}\Delta e+\frac{H}{2L}e,& -L\leq e\leq L\\
    H,& e>L\\
    \end{cases}
\end{split}
\end{equation}
Since the control signal is a linear combination of $\Delta e$ and $e$ it is an incremental PI controller.

\section{Tables}
\subsection{Aggressive Tracking}
\begin{table}[h]
\centering
\caption{Rule Table A: Aggressive Tracking}
\begin{tabular}{llll}
\toprule
{$e\backslash \Delta e$} & N & Z & P \\
\midrule
N & N & N & N \\
Z & N & P & P \\
P & P & P & P \\
\bottomrule
\end{tabular}
\end{table}
Advantage: Fast response and quick convergence to reference.

Disadvantage: May cause overshoot or oscillation in sensitive systems.


\subsection{Conservative Tracking}
\begin{table}[h]
\centering
\caption{Rule Table B: Conservative Tracking}
\begin{tabular}{llll}
\toprule
{$e\backslash \Delta e$} & N & Z & P \\
\midrule
N & N & Z & Z \\
Z & Z & Z & Z \\
P & Z & Z & P \\
\bottomrule
\end{tabular}
\end{table}
Advantage: Very stable with low overshoot.

Disadvantage: Slow response; possible steady-state error if not tuned well.

\subsection{PD-like(Symmetric)}
\begin{table}[h]
\centering
\caption{Rule Table C: PD-like}
\begin{tabular}{llll}
\toprule
{$e\backslash \Delta e$} & N & Z & P \\
\midrule
N & N & Z & P \\
Z & N & Z & P \\
P & N & Z & P \\
\bottomrule
\end{tabular}
\end{table}
Advantage: Symmetric, general-purpose behavior; good if derivative effect dominates.

Disadvantage: No integral action â†’ steady-state error possible.


\section{Piecewise Linear PI/PD controller with Fuzzy PID}
\begin{table}[h!]
\centering
\caption{IC Region Definitions in $(e(n), \Delta e(n))$ Space}
\begin{tabular}{c|ccc|ccc}
\toprule
Region & $e(n)$ & $\mu_P(e)$ & $\mu_N(e)$ &$\Delta e(n)$ & $\mu_P(\Delta e)$ & $\mu_N(\Delta e)$\\
\midrule
IC1 & $0<e(n)<L$ & $\frac{e+L}{2L}$ & $\frac{-e+L}{2L}$ & $-L\leq\Delta e(n)\leq L$ & $\frac{\Delta e+L}{2L}$ & $\frac{-\Delta e+L}{2L}$\\
IC2 & $-L\leq e(n)\leq L$ & $\frac{e+L}{2L}$ & $\frac{-e+L}{2L}$ & $0<\Delta e(n)<L$ & $\frac{\Delta e+L}{2L}$  & $\frac{-\Delta e+L}{2L}$\\
IC3 & $-L<e(n)<0$ & $\frac{e+L}{2L}$ & $\frac{-e+L}{2L}$ & $-L\leq\Delta e(n)\leq L$ & $\frac{\Delta e+L}{2L}$  & $\frac{-\Delta e+L}{2L}$\\
IC4 & $-L\leq e(n)\leq L$ & $\frac{e+L}{2L}$ & $\frac{-e+L}{2L}$ & $-L<\Delta e(n)<0$ & $\frac{\Delta e+L}{2L}$  & $\frac{-\Delta e+L}{2L}$\\
IC5 & $e(n)>L$ & $1$  & $0$ & $-L<\Delta e(n)<0$ & $\frac{\Delta e+L}{2L}$  & $\frac{-\Delta e+L}{2L}$\\
IC6 & $e(n)>L$ & $1$ & $0$ & $\Delta e(n)>L$ & $1$ & $0$\\
IC7 & $-L\leq e(n)\leq L$ & $\frac{e+L}{2L}$  & $\frac{-e+L}{2L}$ & $\Delta e(n)>L$ & $1$ & $0$\\
IC8 & $e<-L$ & $0$ & $1$ & $\Delta e(n)>L$ & $1$ & $0$\\
IC9 & $e<-L$ & $0$& $1$   & $-L<\Delta e(n)<0$ & $\frac{\Delta e+L}{2L}$ & $\frac{-\Delta e+L}{2L}$\\
IC10 & $e<-L$ & $0$& $1$   & $\Delta e(n)<-L$ & $0$ & $1$\\
IC11 & $-L\leq e(n)\leq L$ & $\frac{e+L}{2L}$  & $\frac{-e+L}{2L}$  & $\Delta e(n)<-L$ & $0$ & $1$\\
IC12 & $e(n)>L$ & $1$ & $0$ & $\Delta e(n)<-L$ & $0$ & $1$\\
\bottomrule
\end{tabular}
\end{table}

IC1 
\begin{equation}
\begin{split}
    r1&=\min{\left(\frac{e+L}{2L}_{0<e(n)<L},\frac{\Delta e+L}{2L}_{-L\leq\Delta e(n)\leq L}\right)}\\
    r1&=\frac{\Delta e+L}{2L}_{-L\leq\Delta e(n)\leq L}\\
    r4&=\min{\left(\frac{-e+L}{2L}_{0<e(n)<L},\frac{-\Delta e+L}{2L}_{-L\leq\Delta e(n)\leq L}\right)}\\
    r4&=\frac{-e+L}{2L}_{0<e(n)<L}\\
    u&=Hr_1-Hr_4\\
    u&=H\frac{\Delta e+L}{2L}-H\frac{-e+L}{2L}\\
    u&=\frac{H\Delta e+HL+He-HL}{2L}\\
    u&=\frac{H}{2L}\Delta e+\frac{H}{2L}e
\end{split}
\end{equation}

IC2
\begin{equation}
\begin{split}
    r1&=\min{\left(\frac{e+L}{2L}_{-L\leq e(n)\leq L},\frac{\Delta e+L}{2L}_{0<\Delta e(n)<L}\right)}\\
    r1&=\frac{e+L}{2L}_{-L\leq e(n)\leq L}\\
    r4&=\min{\left(\frac{-e+L}{2L}_{-L\leq e(n)\leq L},\frac{-\Delta e+L}{2L}_{0<\Delta e(n)<L}\right)}\\
    r4&=\frac{-\Delta e+L}{2L}_{0<\Delta e(n)<L}
\end{split}
\end{equation}


IC3
\begin{equation}
\begin{split}
    r1&=\min{\left(\frac{e+L}{2L}_{-L<e(n)<0},\frac{\Delta e+L}{2L}_{-L\leq e(n)\leq L}\right)}\\
    r1&=\frac{e+L}{2L}_{-L<e(n)<0}\\
    r4&=\min{\left(\frac{-e+L}{2L}_{-L\leq e(n)<0},\frac{-\Delta e+L}{2L}_{-L\leq e(n)\leq L}\right)}\\
    r4&=\frac{-\Delta e+L}{2L}_{-L\leq e(n)\leq L}
\end{split}
\end{equation}

IC4
\begin{equation}
\begin{split}
    r1&=\min{\left(\frac{e+L}{2L}_{-L\leq e(n)\leq L},\frac{\Delta e+L}{2L}_{-L<\Delta e(n)<0}\right)}\\
    r1&=\frac{\Delta e+L}{2L}_{-L<\Delta e(n)<0}\\
    r4&=\min{\left(\frac{-e+L}{2L}_{-L\leq e(n)\leq L},\frac{-\Delta e+L}{2L}_{-L<\Delta e(n)<0}\right)}\\
    r4&=\frac{-e+L}{2L}_{-L\leq e(n)\leq L}
\end{split}
\end{equation}

IC5
\begin{equation}
\begin{split}
    r1&=\min{\left(1_{e(n)>L},\frac{\Delta e+L}{2L}_{-L<\Delta e(n)<0}\right)}\\
    r1&=\frac{\Delta e+L}{2L}_{-L<\Delta e(n)<0}\\
    r4&=\min{\left(0_{e(n)>L},\frac{-\Delta e+L}{2L}_{-L<\Delta e(n)<0}\right)}\\
    r4&=0\\
    u&=Hr_1-Hr_4\\
    u&=H\frac{\Delta e+L}{2L}\\
    u&=H\frac{\Delta e}{2L}+H\frac{L}{2L}\\
    u&=\frac{H}{2L}\Delta e+\frac{H}{2}
\end{split}
\end{equation}

IC6
\begin{equation}
\begin{split}
    r1&=\min{\left(1_{e(n)>L},1_{e(n)>L}\right)}\\
    r1&=1\\
    r4&=\min{\left(0_{e(n)>L},0_{e(n)>L}\right)}\\
    r4&=0\\
    u&=H
\end{split}
\end{equation}

IC7
\begin{equation}
\begin{split}
    r1&=\min{\left(\frac{e+L}{2L}_{-L\leq e(n)\leq L},1_{e(n)>L}\right)}\\
    r1&=\frac{e+L}{2L}_{-L\leq e(n)\leq L}\\
    r4&=\min{\left(\frac{-e+L}{2L}_{-L\leq e(n)\leq L},0_{e(n)>L}\right)}\\
    r4&=0\\
    u&=H\frac{e+L}{2L}\\
    u&=\frac{H}{2L}e+\frac{H}{2}
\end{split}
\end{equation}

IC8
\begin{equation}
\begin{split}
    r1&=\min{\left(0_{e<-L},1_{e(n)>L}\right)}\\
    r1&=0\\
    r4&=\min{\left(1_{e<-L},0_{e(n)>L}\right)}\\
    r4&=0\\
    u&=0
\end{split}
\end{equation}

IC9
\begin{equation}
\begin{split}
    r1&=\min{\left(0_{e<-L},\frac{\Delta e+L}{2L}_{-L<\Delta e(n)<0}\right)}\\
    r1&=0\\
    r4&=\min{\left(1_{e<-L},\frac{-\Delta e+L}{2L}_{-L<\Delta e(n)<0}\right)}\\
    r4&=\frac{-\Delta e+L}{2L}_{-L<\Delta e(n)<0}\\
    u&=Hr_1-Hr_4\\
    u&=\frac{H\Delta e-HL}{2L}\\
    u&=\frac{H}{2L}\Delta e-\frac{H}{2}
\end{split}
\end{equation}

IC10
\begin{equation}
\begin{split}
    r1&=\min{\left(0_{e<-L},0_{\Delta e(n)<-L}\right)}\\
    r1&=0\\
    r4&=\min{\left(1_{e<-L},1_{\Delta e(n)<-L}\right)}\\
    r4&=1\\
    u&=Hr_1-Hr_4\\
    u&=-H
\end{split}
\end{equation}

IC11
\begin{equation}
\begin{split}
    r1&=\min{\left(\frac{e+L}{2L}_{-L\leq e(n)\leq L},0_{\Delta e(n)<-L}\right)}\\
    r1&=0\\
    r4&=\min{\left(\frac{-e+L}{2L}_{-L\leq e(n)\leq L},1_{\Delta e(n)<-L}\right)}\\
    r4&=\frac{-e+L}{2L}_{-L\leq e(n)\leq L}\\
    u&=\frac{H}{2L}e-\frac{H}{2}
\end{split}
\end{equation}

IC12
\begin{equation}
\begin{split}
    r1&=\min{\left(1_{e(n)>L},0_{\Delta e(n)<-L}\right)}\\
    r1&=0\\
    r4&=\min{\left(0_{e(n)>L},1_{\Delta e(n)<-L}\right)}\\
    r4&=0\\
    u&=0
\end{split}
\end{equation}



% \begin{table}[h!]
% \centering
% \caption{IC Region Definitions in $(e(n), \Delta e(n))$ Space}
% \begin{tabular}{ccccc}
% \toprule
% Region & r1:$PP$ & r2:$PN$ & r3:$NP$ &r4:$NN$\\
% \midrule
% IC1 & $\frac{e+L}{2L}\frac{\Delta e+L}{2L}$ & $\frac{e+L}{2L}\frac{-\Delta e+L}{2L}$& $\frac{-e+L}{2L}\frac{\Delta e+L}{2L}$& $\frac{-e+L}{2L}\frac{-\Delta e+L}{2L}$\\
% IC2 & $\frac{e+L}{2L}\frac{\Delta e+L}{2L}$ & $\frac{e+L}{2L}\frac{-\Delta e+L}{2L}$& $\frac{-e+L}{2L}\frac{\Delta e+L}{2L}$& $\frac{-e+L}{2L}\frac{-\Delta e+L}{2L}$\\
% IC3 & $\frac{e+L}{2L}\frac{\Delta e+L}{2L}$ & $\frac{e+L}{2L}\frac{-\Delta e+L}{2L}$& $\frac{-e+L}{2L}\frac{\Delta e+L}{2L}$& $\frac{-e+L}{2L}\frac{-\Delta e+L}{2L}$\\
% IC4 & $\frac{e+L}{2L}\frac{\Delta e+L}{2L}$ & $\frac{e+L}{2L}\frac{-\Delta e+L}{2L}$& $\frac{-e+L}{2L}\frac{\Delta e+L}{2L}$& $\frac{-e+L}{2L}\frac{-\Delta e+L}{2L}$\\
% \bottomrule
% \end{tabular}
% \end{table}